New version of Babel Light Protocol (hmac nonce)

babel_light.v
@@ -27,10 +27,10 @@
         b -> a  : Literal([TagMsg]) | msg
         a       : assert(Msg(a, b, msg))
         a       : Log(ChallengeRequest(a, b, n0, msg))
-        a -> b  : Literal([TagChallengeRequest]) | msg | n0
+        a -> b  : Literal([TagChallengeRequest]) | msg | hmac(k, n0)
         b       : assert(ChallengeRequest(a, b, n0, msg))
         b       : Log(ChallengeReply(a, b, n0))
-        b -> a  : Literal([TagChallengeReply]) | n0
+        b -> a  : Literal([TagChallengeReply]) | hmac(k, n0)
         a       : assert(ChallengeReply(a, b, msg, n0))
 *)
 
@@ -40,12 +40,14 @@ Require Import ListSet.
 
 Inductive term: Type :=
     | Literal (b: string)
-    | Pair (a: term) (b: term).
+    | Pair (a: term) (b: term)
+    | HMac (k: term) (p: term).
 
 (* Signature: Protocol Usages and Events *)
 
 Module Type ProtocolDefs.
     Parameter nonce_usage: Type.
+    Parameter hmac_usage: Type.
     Parameter pEvent: Type.
 End ProtocolDefs.
 
@@ -62,6 +64,10 @@ Module BabelLightDefs <: ProtocolDefs.
         | ChallengeReply (a b msg: term).
     Definition nonce_usage := nonce_usage'.
 
+    Inductive hmac_usage' :=
+        | HNonce (n: term).
+    Definition hmac_usage := hmac_usage'.
+    
     Inductive pEvent' :=
         | Msg (a b msg : term)
         | Request (a b n0 msg: term)
@@ -75,7 +81,8 @@ Module Defs (PD : ProtocolDefs).
 
     Inductive usage: Type :=
         | AdversaryGuess
-        | Nonce (nu: nonce_usage).
+        | Nonce (nu: nonce_usage)
+        | HMacKey (hu: hmac_usage).
 
     Inductive event: Type :=
         | New (t: term) (u: usage)
@@ -104,12 +111,11 @@ Module Type ProtocolInvariants (PD: ProtocolDefs).
     
     Parameter LogInvariant: log -> Prop.
 
-    (* Nonce Predicate *)
-    Parameter nonceComp: term -> log -> Prop.
-    Parameter nonceComp_Stable: forall t, Stable (nonceComp t).
+    Parameter hmacComp : term -> log -> Prop.
+    Parameter hmacComp_Stable: forall t, Stable (hmacComp t).
 
-    (*Parameter canNonce : term -> term -> log -> Prop.
-    Parameter canNonce_Stable: forall n m, Stable (canNonce n m).*)
+    Parameter canHmac : term -> term -> log -> Prop.
+    Parameter canHmac_Stable: forall k n, Stable (canHmac k n).
 End ProtocolInvariants.
 
 Module BabelLightInvariants <: ProtocolInvariants BabelLightDefs.
@@ -118,91 +124,43 @@ Module BabelLightInvariants <: ProtocolInvariants BabelLightDefs.
 
     Definition LogInvariant L :=
         forall t u, Logged (New t u) L -> (exists bs, t = Literal bs).
+    
+    Definition RequestN a b k msg L :=
+        exists n, Logged (New k (HMacKey (HNonce n))) L /\ Logged (New n (Nonce (ChallengeRequest a b msg))) L.
+    
+    Definition ResponseN a b k msg L := 
+        exists n, Logged (New k (HMacKey (HNonce n))) L /\ Logged (New n (Nonce (ChallengeReply a b msg))) L.
 
-    Definition RequestNComp a b L :=
+    Definition keyComp a b L :=
         LoggedP (Bad a) L \/ LoggedP (Bad b) L.
-    
-    Definition RequestN a b n msg L :=
-        Logged (New n (Nonce (ChallengeRequest a b msg))) L.
 
-    Definition ResponseNComp a b L := 
-        LoggedP (Bad a) L \/ LoggedP (Bad b) L.
-    
-    Definition ResponseN a b n msg L := 
-        Logged (New n (Nonce (ChallengeReply a b msg))) L.
-        
-    Definition nonceComp n L := 
-        exists a, exists b, exists msg, (RequestN a b n msg L /\ RequestNComp a b L)
-            \/ (ResponseN a b n msg L /\ ResponseNComp a b L).
+    Definition hmacComp k L :=
+        exists a, exists b, exists msg, (RequestN a b k msg L \/ ResponseN a b k msg L) /\ keyComp a b L.
 
-    Definition nonceComp_Stable:
-        forall t, Stable (nonceComp t).
+    Theorem hmacComp_Stable:
+        forall t, Stable (hmacComp t).
+    Admitted.
+
+    Definition noncePayload a b n L :=
+        (exists msg, exists p, exists k, 
+            p = Pair (Literal (String TagChallengeRequest EmptyString)) (Pair msg (HMac k n)) /\
+            LoggedP (Request a b n msg) L) \/
+        (exists p, exists msg, exists k,
+            p = Pair (Literal (String TagChallengeReply EmptyString)) (HMac k n) /\
+            LoggedP (Reply a b n msg) L).
+
+    Definition canHmac k n L :=
+        exists a, exists b, exists msg, (RequestN a b k msg L \/ ResponseN a b k msg L) /\ noncePayload a b n L.
+
+    Theorem canHmac_Stable:
+        forall k n, Stable (canHmac k n).
     Proof.
-        intro t. unfold Stable. intros L L'.
-        unfold leq_log. unfold nonceComp. unfold RequestN. unfold RequestNComp.
-        unfold ResponseN. unfold ResponseNComp. unfold LoggedP.
-        intros Hleq_log HnonceCompL. destruct HnonceCompL as (a, HnonceCompL_a).
-        destruct HnonceCompL_a as (b, HnonceCompL_ab). destruct HnonceCompL_ab as (msg, HnonceCompL_abmsg).
-        exists a. exists b. exists msg. firstorder.
-    Qed.   
-
-    Definition RequestAB a b n msg L :=
-        Logged (New n (Nonce (ChallengeRequest a b msg))) L.
-
-    Definition ResponseAB a b n msg L :=
-        Logged (New n (Nonce (ChallengeReply a b msg))) L. 
-
-    (*Definition ExchangeAB a b n0 msg L :=
-        Logged (New n0 (Nonce_U (Challenge a b msg))) L.
-
-    Definition ExchangeABComp p L :=
-        LoggedP (Bad p) L.
-
-    Definition nonceComp n0 L :=
-        exists a, exists b, exists msg, ExchangeAB a b n0 msg L /\ ExchangeABComp a L.
-
-    Theorem nonceComp_Stable:
-        forall n0, Stable (nonceComp n0).
-    Proof.
-        intro n0. unfold Stable. intros L L'.
-        unfold leq_log. unfold nonceComp. unfold ExchangeAB. unfold ExchangeABComp. unfold LoggedP.
-        intros Hleq_log HlogL.
-        destruct HlogL as (a, HlogL_a). destruct HlogL_a as (b, HlogL_ab). destruct HlogL_ab as (msg, HlogL_abmsg).
-        destruct HlogL_abmsg as (HlogL_abmsg_nonce & HlogL_abmsg_bad).
-        exists a. exists b. exists msg. split.
-        - specialize Hleq_log with (e:=New n0 (Nonce_U (Challenge a b msg))). apply Hleq_log. assumption.
-        - specialize Hleq_log with (e:=ProtEvent (Bad a)). apply Hleq_log. assumption.
-    Qed.
-
-    Definition ExchangeABPayload a b p L :=
-        (exists n0, exists msg,
-            p = Pair (Literal (String TagChallengeRequest EmptyString)) (Pair n0 msg) /\
-            LoggedP (ChallengeRequest a b n0 msg) L
-        ) \/
-        (exists n0,
-            p = Pair (Literal (String TagChallengeReply EmptyString)) n0 /\
-            LoggedP (ChallengeReply a b n0) L
-        ).
-    
-    Definition canNonce n p L :=
-        exists a, exists b, exists msg, ExchangeAB a b n msg L /\ ExchangeABPayload a b p L.
-
-    Theorem canNonce_Stable:
-        forall n p, Stable (canNonce n p).
-    Proof.
-        intros n p. unfold Stable. intros L L'.
-        unfold leq_log. unfold canNonce. unfold ExchangeAB. unfold ExchangeABPayload. unfold LoggedP.
-        intros Hleq_log HlogL. destruct HlogL as (a, HlogL_a). destruct HlogL_a as (b, HlogL_ab). destruct HlogL_ab as (msg, HlogL_abmsg).
-        exists a. exists b. exists msg.
-        destruct HlogL_abmsg as (HlogL_abmsg_ExchAB & HlogL_abmsg_ExchABPayload). split.
-        - specialize Hleq_log with (e:=New n (Nonce_U (Challenge a b msg))). apply Hleq_log. assumption.
-        - destruct HlogL_abmsg_ExchABPayload as [HlogL_abmsg_EABP_req | HlogL_abmsg_EABP_resp].
-            * left. destruct HlogL_abmsg_EABP_req as (n0, HlogL_abmsg_EABP_req_n0). 
-                destruct HlogL_abmsg_EABP_req_n0 as (msg0, HlogL_abmsg_EABP_req_n0msg).
-                exists n0. exists msg0. firstorder.
-            * right. destruct HlogL_abmsg_EABP_resp as (n0, HlogL_abmsg_EABP_resp_n0).
-                exists n0. firstorder.
-    Qed.*)
+        intros k n. unfold Stable. intros L L'. unfold leq_log. unfold canHmac.
+        unfold RequestN. unfold ResponseN. unfold noncePayload. unfold LoggedP.
+        intros Hleq_log HcanHmacL. destruct HcanHmacL as (a, HcanHmacL_a).
+        destruct HcanHmacL_a as (b, HcanHmacL_ab). destruct HcanHmacL_ab as (msg, HcanHmacL_abmsg).
+        exists a. exists b. exists msg. 
+    Admitted.
 End BabelLightInvariants.
 
 Module CryptographicInvariants (PD: ProtocolDefs) (PI: ProtocolInvariants PD).
@@ -217,24 +175,15 @@ Module CryptographicInvariants (PD: ProtocolDefs) (PI: ProtocolInvariants PD).
             Logged (New (Literal bs) AdversaryGuess) L ->
             Level l (Literal bs) L
 
-        | Level_Nonce: forall l bs L nu,
-            Logged (New (Literal bs) (Nonce nu)) L ->
-            (l = Low -> nonceComp (Literal bs) L) ->
-            Level l (Literal bs) L 
-
         | Level_Pair: forall l t1 t2 L,
             Level l t1 L ->
             Level l t2 L ->
             Level l (Pair t1 t2) L
             
-        (*| Level_NonceU: forall l n m L,
-            canNonce n m L ->
+        | Level_HMac: forall l k n L,
+            canHmac k n L ->
             Level l m L ->
-            Level l (Nonce n m) L
-        | Level_NonceU_Low: forall l n m L,
-            Level Low n L ->
-            Level Low m L ->
-            Level l (Nonce n m) L*).
+            Level l (HMac k n).
     
     Theorem Low_High: forall t L,
         Level Low t L -> Level High t L.
@@ -244,8 +193,6 @@ Module CryptographicInvariants (PD: ProtocolDefs) (PI: ProtocolInvariants PD).
         - apply Level_AdversaryGuess. assumption.
         - apply Level_Nonce with (nu:=nu) ; try assumption. easy.
         - apply Level_Pair ; assumption.
-        (*- apply Level_NonceU ; assumption.
-        - apply Level_NonceU_Low ; assumption.*)
     Qed.
 
     Theorem Level_Stable: forall l t L L',
@@ -262,9 +209,6 @@ Module CryptographicInvariants (PD: ProtocolDefs) (PI: ProtocolInvariants PD).
             * intro Hllow. apply H0 in Hllow. 
                 assert ( Hstable : Stable (nonceComp (Literal bs)) ). apply nonceComp_Stable. firstorder.
         - apply Level_Pair ; firstorder.
-        (*- apply Level_NonceU ; try auto.
-            assert ( HStable : Stable (canNonce n m) ). apply canNonce_Stable. firstorder.
-        - apply Level_NonceU_Low ; firstorder.*)
     Qed.
 
     Theorem AbsurdDistinctUsages : forall P L t u u',
@@ -281,220 +225,8 @@ Module CryptographicInvariants (PD: ProtocolDefs) (PI: ProtocolInvariants PD).
         apply HGL_WfLog in HlogU ; try assumption.
         exfalso. tauto.
     Qed.
-
-    Theorem LowNonce_Inversion : forall L n nu,
-        GoodLog L ->
-        Logged (New (Literal n) (Nonce nu)) L ->
-        forall l t, l = Low -> t = Literal n -> Level l t L ->
-        nonceComp (Literal n) L.
-    Proof.
-        intros L n nu. intros HGoodLog Hlog. intros l t. intros Hlow HLit Hlevel. symmetry in HLit.
-        unfold GoodLog in HGoodLog. destruct HGoodLog as (HGL_WfLog & _).
-        unfold WF_Log in HGL_WfLog.
-        induction Hlevel ; try discriminate. 
-        - exfalso. specialize HGL_WfLog with (t:=Literal n) (u:=Nonce nu) (u':=AdversaryGuess).
-            apply HGL_WfLog in Hlog ; try assumption. 
-            + discriminate. 
-            + rewrite HLit. assumption. 
-        - apply H0 in Hlow. rewrite <- HLit in Hlow. assumption.
-    Qed.
-
-    Theorem LowPair_Inversion: forall L t1 t2,
-        GoodLog L ->
-        forall l t, l = Low -> t = Pair t1 t2 -> Level l t L ->
-        Level Low t1 L /\ Level Low t2 L.
-    Proof.
-        intros L t1 t2. intro HGoodLog. intros l t. intros Hlow Hterm Hlevel.
-        unfold GoodLog in HGoodLog. destruct HGoodLog as (HGL_WfLog & _).
-        unfold WF_Log in HGL_WfLog.
-        induction Hlevel ; try discriminate. 
-        injection Hterm. intros Ht3 Ht0. split.
-        - rewrite Hlow in Hlevel1. rewrite Ht0 in Hlevel1. assumption.
-        - rewrite Hlow in Hlevel2. rewrite Ht3 in Hlevel2. assumption.
-    Qed.
-
-    (*Theorem Nonce_Inversion : forall L l n m,
-        forall t, t = Nonce n m -> Level l t L ->
-        canNonce n m L \/ Level Low n L.
-    Proof.
-        intros L l n m. intro t. intros Hnonce Hlevel.
-        induction Hlevel ; try discriminate.
-        - left. injection Hnonce. intros Hm0 Hn0. rewrite Hm0 in H. rewrite Hn0 in H. assumption.
-        - right. injection Hnonce. intros _ Hn0. rewrite Hn0 in Hlevel1. assumption.
-    Qed.*)
 End CryptographicInvariants.
 
 Import BabelLightDefs.
 Include CryptographicInvariants BabelLightDefs BabelLightInvariants.
 Import BabelLightInvariants.
-
-Theorem ChallengeRequestCorrespondence: forall a b n0 msg L,
-    GoodLog L -> RequestAB a b n0 msg L ->
-    forall l t, l = Low -> t = Pair (Literal (String TagChallengeRequest EmptyString)) (Pair n0 msg) ->
-    Level l t L -> LoggedP (Request a b n0 msg) L \/ (LoggedP (Bad a) L \/ LoggedP (Bad b) L).
-Proof.
-    intros a b n0 msg L. unfold RequestAB. intros HGoodLog Hrequest. intros l t. intros Hlow Hterm Hlevel.
-    assert ( HGoodLog_bis : GoodLog L ). assumption.
-    unfold GoodLog in HGoodLog. destruct HGoodLog as (HGL_WfLog & HGL_LogInv).
-    unfold WF_Log in HGL_WfLog. unfold LogInvariant in HGL_LogInv.
-    induction Hlevel ; try discriminate. injection Hterm. intros Ht2 Ht1.
-    assert ( Hrequest_bis : Logged (New n0 (Nonce (ChallengeRequest a b msg))) L ). assumption.
-    specialize HGL_LogInv with (t:=n0) (u:=Nonce (ChallengeRequest a b msg)). apply HGL_LogInv in Hrequest_bis.
-    destruct Hrequest_bis as (bs, HLitn0). assert ( HnonceComp : nonceComp (Literal bs) L ).
-    - apply LowNonce_Inversion with (t:=Literal bs) (l:=Low) (nu:=ChallengeRequest a b msg) ; try easy.
-        + rewrite HLitn0 in Hrequest. assumption.
-        + rewrite Ht2 in Hlevel2. rewrite Hlow in Hlevel2.
-            assert ( Hpair : Level Low (Literal bs) L /\ Level Low msg L ).
-            *  apply LowPair_Inversion with (t1:=Literal bs) (t2:=msg) (l:= Low) (t:=Pair (Literal bs) msg) ; try easy.
-                rewrite HLitn0 in Hlevel2. assumption.
-            * destruct Hpair as (Hpair & _). assumption.
-    - unfold nonceComp in HnonceComp. destruct HnonceComp as (a0, HnonceComp_a).
-        destruct HnonceComp_a as (b0, HnonceComp_ab). destruct HnonceComp_ab as (msg0, HnonceComp_abmsg).
-        destruct HnonceComp_abmsg as [HNC_request | HNC_response].
-        + destruct HNC_request as (HNC_request_req & HNC_request_reqComp).
-            unfold RequestN in HNC_request_req. unfold RequestNComp in HNC_request_reqComp.
-            rewrite HLitn0 in Hrequest. 
-            specialize HGL_WfLog with (t:=Literal bs) (u:=Nonce (ChallengeRequest a b msg)) (u':=Nonce (ChallengeRequest a0 b0 msg0)).
-            apply HGL_WfLog in Hrequest ; try assumption. injection Hrequest. intros _ Hb Ha. 
-            rewrite <- Ha in HNC_request_reqComp. rewrite <- Hb in HNC_request_reqComp.
-            right. assumption.
-        + destruct HNC_response as (HNC_response_resp & _). unfold ResponseN in HNC_response_resp.
-            rewrite HLitn0 in Hrequest. 
-            specialize HGL_WfLog with (t:=Literal bs) (u:=Nonce (ChallengeRequest a b msg)) (u':=Nonce (ChallengeReply a0 b0 msg0)).
-            apply HGL_WfLog in Hrequest ; try assumption. discriminate.
-Qed.
-
-Theorem ChallengeReplyCorrespondence: forall a b n0 msg L,
-    GoodLog L -> ResponseAB a b n0 msg L ->
-    forall l t, l = Low -> t = Pair (Literal (String TagChallengeReply EmptyString)) n0 ->
-    Level l t L -> LoggedP (Reply a b n0 msg) L \/ (LoggedP (Bad a) L \/ LoggedP (Bad b) L).
-Proof.
-    intros a b n0 msg L. unfold ResponseAB. intros HGoodLog Hresponse. intros l t. intros Hlow Hterm Hlevel.
-    assert ( HGoodLog_bis : GoodLog L ). assumption.
-    unfold GoodLog in HGoodLog. destruct HGoodLog as (HGL_WfLog & HGL_LogInv).
-    unfold WF_Log in HGL_WfLog. unfold LogInvariant in HGL_LogInv.
-    induction Hlevel ; try discriminate. injection Hterm. intros Ht2 Ht1.
-    assert ( Hresponse_bis : Logged (New n0 (Nonce (ChallengeReply a b msg))) L ). assumption.
-    specialize HGL_LogInv with (t:=n0) (u:=Nonce (ChallengeReply a b msg)). apply HGL_LogInv in Hresponse_bis.
-    destruct Hresponse_bis as (bs, HLitn0). assert ( HnonceComp : nonceComp (Literal bs) L ).
-    - apply LowNonce_Inversion with (t:=Literal bs) (l:=Low) (nu:=ChallengeReply a b msg) ; try easy.
-        + rewrite HLitn0 in Hresponse. assumption.
-        + rewrite Hlow in Hlevel2. rewrite Ht2 in Hlevel2. rewrite HLitn0 in Hlevel2. assumption.
-    - unfold nonceComp in HnonceComp. destruct HnonceComp as (a0, HnonceComp_a). 
-        destruct HnonceComp_a as (b0, HnonceComp_ab). destruct HnonceComp_ab as (msg0, HnonceComp_abmsg).
-        destruct HnonceComp_abmsg as [HNC_request | HNC_response].
-        + destruct HNC_request as (HNC_request_req & _). unfold RequestN in HNC_request_req.
-            rewrite HLitn0 in Hresponse. 
-            specialize HGL_WfLog with (t:=Literal bs) (u:=Nonce (ChallengeReply a b msg)) (u':=Nonce (ChallengeRequest a0 b0 msg0)).
-            apply HGL_WfLog in Hresponse ; try assumption. discriminate.
-        + destruct HNC_response as (HNC_response_resp & HNC_response_respComp). 
-            unfold ResponseN in HNC_response_resp. unfold ResponseNComp in HNC_response_respComp. rewrite HLitn0 in Hresponse.
-            specialize HGL_WfLog with (t:=Literal bs) (u:=Nonce (ChallengeReply a b msg)) (u':=Nonce (ChallengeReply a0 b0 msg0)).
-            apply HGL_WfLog in Hresponse ; try assumption. injection Hresponse. intros _ Hb Ha.
-            rewrite <- Ha in HNC_response_respComp. rewrite <- Hb in HNC_response_respComp.
-            right. assumption.
-Qed.
-
-(*Theorem ChallengeRequestCorrespondence: forall a b n0 msg L,
-    GoodLog L -> ExchangeAB a b n0 msg L ->
-    forall l t, l = Low -> t = Nonce n0 (Pair (Literal (String TagChallengeRequest EmptyString)) (Pair n0 msg)) ->
-    Level l t L -> LoggedP (ChallengeRequest a b n0 msg) L \/ LoggedP (Bad a) L.
-Proof.
-    intros a b n0 msg L. unfold ExchangeAB.
-    intros HGoodLog HExchangeAB. intros l t. intros Hlow Hnonce Hlevel.
-    assert ( HGoodLog_bis : GoodLog L ). assumption.
-    unfold GoodLog in HGoodLog. destruct HGoodLog as (HGL_WfLog & HGL_LogInv).
-    unfold WF_Log in HGL_WfLog. unfold LogInvariant in HGL_LogInv. induction Hlevel ; try discriminate.
-    - left. injection Hnonce. intros Hm Hn. rewrite Hn in H. unfold canNonce in H.
-        destruct H as (a0, Ha). destruct Ha as (b0, Hab). destruct Hab as (msg0, Habmsg).
-        destruct Habmsg as (Habmsg_ExchAB & Habmsg_ExchABPayload). unfold ExchangeAB in Habmsg_ExchAB.
-        specialize HGL_WfLog with (t:=n0) (u:=Nonce_U (Challenge a b msg)) (u':=Nonce_U (Challenge a0 b0 msg0)).
-        apply HGL_WfLog in Habmsg_ExchAB ; try assumption. injection Habmsg_ExchAB.
-        intros Hmsg Hb Ha. unfold ExchangeABPayload in Habmsg_ExchABPayload.
-        destruct Habmsg_ExchABPayload as [Habmsg_EABP_req | Habmsg_EABP_resp].
-        + destruct Habmsg_EABP_req as (n', Habmsg_EABP_req_n0). destruct Habmsg_EABP_req_n0 as (msg', Habmsg_EABP_req_n0msg).
-            destruct Habmsg_EABP_req_n0msg as (Habmsg_EABP_req_msg & Habmsg_EABP_req_log).
-            symmetry in Habmsg_EABP_req_msg. rewrite Hm in Habmsg_EABP_req_msg. injection Habmsg_EABP_req_msg.
-            intros Hmsg' Hn'. rewrite Ha. rewrite Hb. rewrite Hn' in Habmsg_EABP_req_log. rewrite Hmsg' in Habmsg_EABP_req_log.
-            assumption.
-        + exfalso. destruct Habmsg_EABP_resp as (n', Habmsg_EABP_resp_n0).
-            destruct Habmsg_EABP_resp_n0 as (Habmsg_EABP_resp_msg & _). symmetry in Habmsg_EABP_resp_msg. 
-            rewrite Hm in Habmsg_EABP_resp_msg. injection Habmsg_EABP_resp_msg. intros _ Htag.
-            assert ( HtagDistinct : TagChallengeRequest <> TagChallengeReply ). apply TagsDistinct. firstorder.
-    - right. injection Hnonce. intros Hm Hn.
-        specialize HGL_LogInv with (t:=n0) (u:=Nonce_U (Challenge a b msg)).
-        assert ( Hlog : Logged (New n0 (Nonce_U (Challenge a b msg))) L ). assumption.
-        apply HGL_LogInv in HExchangeAB. destruct HExchangeAB as (bs, HLitn0).
-        assert ( HnonceComp : nonceComp (Literal bs) L ).
-        + apply LowNonce_Inversion with (nu:=Challenge a b msg) (l:=Low) (t:=Literal bs) ; try easy.
-            * rewrite HLitn0 in Hlog. assumption.
-            * rewrite Hn in Hlevel1. rewrite HLitn0 in Hlevel1. assumption.
-        + unfold nonceComp in HnonceComp. destruct HnonceComp as (a0, HnonceComp_a). destruct HnonceComp_a as (b0, HnonceComp_ab).
-            destruct HnonceComp_ab as (msg0, HnonceComp_abmsg). destruct HnonceComp_abmsg as (HnonceComp_ExchAB & HnonceComp_ExchABComp).
-            unfold ExchangeAB in HnonceComp_ExchAB. rewrite HLitn0 in Hlog. 
-            specialize HGL_WfLog with (t:=Literal bs) (u:=Nonce_U (Challenge a b msg)) (u':=Nonce_U (Challenge a0 b0 msg0)).
-            apply HGL_WfLog in Hlog ; try assumption. injection Hlog. intros Hmsg Hb Ha.
-            unfold ExchangeABComp in HnonceComp_ExchABComp. rewrite Ha. assumption.
-Qed.
-
-Theorem ChallengeReplyCorrespondence: forall a b n0 msg L,
-    GoodLog L -> ExchangeAB a b n0 msg L ->
-    forall l t, l = Low -> t = Nonce n0 (Pair (Literal (String TagChallengeReply EmptyString)) n0) ->
-    Level l t L -> LoggedP (ChallengeReply a b n0) L \/ LoggedP (Bad a) L.
-Proof.
-    intros a b n0 msg L. unfold ExchangeAB. 
-    intros HGoodLog HExchangeAB. intros l t. intros Hlow Hnonce Hlevel.
-    assert ( HGoodLog_bis : GoodLog L ). assumption.
-    unfold GoodLog in HGoodLog. destruct HGoodLog as (HGL_WfLog & HGL_LogInv).
-    unfold WF_Log in HGL_WfLog. unfold LogInvariant in HGL_LogInv. 
-    induction Hlevel ; try discriminate.
-    - left. injection Hnonce. intros Hm Hn. unfold canNonce in H. destruct H as (a0, Ha).
-        destruct Ha as (b0, Hab). destruct Hab as (msg0, Habmsg). destruct Habmsg as (Habmsg_ExchAB & Habmsg_ExchABPayload).
-        unfold ExchangeAB in Habmsg_ExchAB. rewrite Hn in Habmsg_ExchAB.
-        specialize HGL_WfLog with (t:=n0) (u:=Nonce_U (Challenge a b msg)) (u':=Nonce_U (Challenge a0 b0 msg0)).
-        apply HGL_WfLog in HExchangeAB ; try assumption. injection HExchangeAB. intros Hmsg Hb Ha. unfold ExchangeABPayload in Habmsg_ExchABPayload.
-        destruct Habmsg_ExchABPayload as [Habmsg_EABP_req | Habmsg_EABP_resp].
-        * exfalso. destruct Habmsg_EABP_req as (n', Habmsg_EABP_req_n0). destruct Habmsg_EABP_req_n0 as (msg', Habmsg_EABP_req_n0msg).
-            destruct Habmsg_EABP_req_n0msg as (Habmsg_EABP_req_msg & _). symmetry in Habmsg_EABP_req_msg.
-            rewrite Hm in Habmsg_EABP_req_msg. injection Habmsg_EABP_req_msg. intros _ Htag.
-            assert ( HtagDistinct : TagChallengeRequest <> TagChallengeReply ). apply TagsDistinct. tauto.
-        * destruct Habmsg_EABP_resp as (n', Habmsg_EABP_resp_n0). destruct Habmsg_EABP_resp_n0 as (Habmsg_EABP_resp_msg & Habmsg_EABP_resp_log).
-            symmetry in Habmsg_EABP_resp_msg. rewrite Hm in Habmsg_EABP_resp_msg. injection Habmsg_EABP_resp_msg.
-            intros Hn'. rewrite Ha. rewrite Hb. rewrite Hn' in Habmsg_EABP_resp_log. assumption.
-    - right. injection Hnonce. intros Hm Hn.
-        specialize HGL_LogInv with (t:=n0) (u:=Nonce_U (Challenge a b msg)).
-        assert ( Hlog : Logged (New n0 (Nonce_U (Challenge a b msg))) L ). assumption.
-        apply HGL_LogInv in HExchangeAB. destruct HExchangeAB as (bs, HLitn0).
-        assert ( HnonceComp : nonceComp (Literal bs) L ).
-        + apply LowNonce_Inversion with (nu:=Challenge a b msg) (l:=Low) (t:=Literal bs) ; try easy.
-            * rewrite HLitn0 in Hlog. assumption.
-            * rewrite Hn in Hlevel1. rewrite HLitn0 in Hlevel1. assumption.
-        + unfold nonceComp in HnonceComp. destruct HnonceComp as (a0, HnonceComp_a). destruct HnonceComp_a as (b0, HnonceComp_ab).
-            destruct HnonceComp_ab as (msg0, HnonceComp_abmsg). destruct HnonceComp_abmsg as (HnonceComp_ExchAB & HnonceComp_ExchABComp).
-            unfold ExchangeAB in HnonceComp_ExchAB. rewrite HLitn0 in Hlog.
-            specialize HGL_WfLog with (t:=Literal bs) (u:=Nonce_U (Challenge a b msg)) (u':=Nonce_U (Challenge a0 b0 msg0)).
-            apply HGL_WfLog in HnonceComp_ExchAB ; try assumption. injection HnonceComp_ExchAB. intros Hmsg Hb Ha.
-            unfold ExchangeABComp in HnonceComp_ExchABComp. rewrite Ha. assumption.
-Qed.
-
-Theorem NonceSecrecy: forall a b n0 msg L,
-    GoodLog L -> ExchangeAB a b n0 msg L ->
-    forall l, l = Low -> Level l n0 L ->
-    LoggedP (Bad a) L.
-Proof.
-    intros a b n0 msg L. unfold ExchangeAB.
-    intros HGoodLog HExchangeAB. intro l. intros Hlow Hlevel.
-    unfold GoodLog in HGoodLog. destruct HGoodLog as (HGL_WfLog & HGL_LogInv).
-    unfold WF_Log in HGL_WfLog. unfold LogInvariant in HGL_LogInv.
-    specialize HGL_LogInv with (t:=n0) (u:=Nonce_U (Challenge a b msg)).
-    assert ( HExchangeAB_bis : Logged (New n0 (Nonce_U (Challenge a b msg))) L ). assumption.
-    apply HGL_LogInv in HExchangeAB_bis. destruct HExchangeAB_bis as (bs, HLitn0).
-    induction n0 ; try discriminate. induction Hlevel ; try discriminate.
-    - specialize HGL_WfLog with (t:=Literal bs0) (u:=Nonce_U (Challenge a b msg)) (u':=AdversaryGuess).
-        apply HGL_WfLog in HExchangeAB ; try assumption. discriminate.
-    - apply H0 in Hlow. unfold nonceComp in Hlow. destruct Hlow as (a', Hlow_a). destruct Hlow_a as (b', Hlow_ab).
-        destruct Hlow_ab as (msg', Hlow_abmsg). destruct Hlow_abmsg as (Hlow_exchAB & Hlow_exchABComp).
-        unfold ExchangeAB in Hlow_exchAB. specialize HGL_WfLog with (t:=Literal bs0) (u:=Nonce_U (Challenge a b msg)) (u':=Nonce_U (Challenge a' b' msg')).
-        apply HGL_WfLog in HExchangeAB ; try assumption. injection HExchangeAB. intros Hmsg Hb Ha.
-        unfold ExchangeABComp in Hlow_exchABComp. rewrite Ha. assumption.
-Qed.*)
